code/experimental/rsa/Convert.fst
@@ -13,69 +13,80 @@ type bignum = buffer FStar.UInt64.t
 
 let bn_bytes = 8ul
 
-(* the length of the message in octets *)
-val get_size_nat: lenText:U32.t -> Tot U32.t
+(* text_to_bn *)
+val get_size_nat: lenText:U32.t{U32.v lenText > 0} -> Tot (res:U32.t{U32.v res > 0})
 let get_size_nat lenText =
-     U32.((lenText -^ 1ul) /^ bn_bytes +^ 1ul)
+    U32.(((lenText -^ 1ul) >>^ 3ul) +^ 1ul)
 
-val bits_to_bn: bits:U32.t -> Tot U32.t
+val bits_to_bn: bits:U32.t{U32.v bits > 0} -> Tot (res:U32.t{U32.v res > 0})
 let bits_to_bn bits =
-    let to_octets = U32.((bits -^ 1ul) /^ 8ul +^ 1ul) in
-    U32.((to_octets -^ 1ul) /^ 8ul +^ 1ul)
+    U32.(((bits -^ 1ul) >>^ 6ul) +^ 1ul)
 
-val bits_to_text: bits:U32.t -> Tot U32.t
+val bits_to_text: bits:U32.t{U32.v bits > 0} -> Tot (res:U32.t{U32.v res > 0})
 let bits_to_text bits =
-    U32.((bits -^ 1ul)/^ 8ul +^ 1ul)
+    U32.(((bits -^ 1ul) >>^ 3ul) +^ 1ul)
 
 val text_to_nat_loop:
-    input:uint8_p -> len:U32.t -> res:bignum ->
-    num_words:U32.t{U32.v num_words <= length res} -> m:U32.t -> word:U64.t ->
+    input:uint8_p -> len:U32.t{U32.v len = length input /\ U32.v len > 0} ->
+    res:bignum{length res = U32.v (get_size_nat len)} ->
+    num_words:U32.t{U32.v num_words <= length res /\ U32.v num_words > 0} ->
+    m:U32.t{0 <= U32.v m /\ U32.v m < 8} -> word:U64.t ->
     i:U32.t{U32.v i <= length input} -> Stack unit
     (requires (fun h -> live h input /\ live h res))
-    (ensures (fun h0 _ h1 -> live h0 input /\ live h0 res /\ live h1 input /\ live h1 res /\ modifies_1 res h0 h1))
+    (ensures (fun h0 _ h1 -> live h0 input /\ live h0 res /\ 
+        live h1 input /\ live h1 res /\ modifies_1 res h0 h1))
+      (* #set-options "--z3rlimit 20" *)
 let rec text_to_nat_loop input len res num_words m word i =
-	if U32.(len >^ 0ul) then
-    let len = U32.(len -^ 1ul) in
-    let tmp = input.(i) in
-	let word = U64.((word <<^ 8ul) |^ uint8_to_uint64 tmp) in
-	let i = U32.(i +^ 1ul) in
-	if U32.(m =^ 0ul) then
-	    let num_words = U32.(num_words -^ 1ul) in
-	    res.(num_words) <- word;
-	    let word = 0uL in
-        let m = U32.(bn_bytes -^ 1ul) in
-	    text_to_nat_loop input len res num_words m word i
-	else
-        text_to_nat_loop input len res num_words U32.(m -^ 1ul) word i
+    (* len = 8 * num_words + m *)
+	if U32.(i <^ len) then
+        begin
+        let tmp = input.(i) in
+	    let word = U64.((word <<^ 8ul) |^ uint8_to_uint64 tmp) in
+	    let i = U32.(i +^ 1ul) in
+        if U32.(m =^ 0ul) then
+	        (let num_words = U32.(num_words -^ 1ul) in
+	        res.(num_words) <- word;
+	        text_to_nat_loop input len res num_words 7ul 0uL i)
+	    else
+            (let m = U32.(m -^ 1ul) in
+            text_to_nat_loop input len res num_words m word i)
+        end
 	else ()
 
 val text_to_nat:
-    input:uint8_p -> len:U32.t{U32.v len = length input} -> res:bignum -> Stack unit
+    input:uint8_p -> len:U32.t{U32.v len = length input /\ U32.v len > 0} ->
+    res:bignum{length res = U32.v (get_size_nat len)} -> Stack unit
 	(requires (fun h -> live h input /\ live h res))
-	(ensures (fun h0 _ h1 -> live h0 input /\ live h0 res /\ live h1 res /\ modifies_1 res h0 h1))
+	(ensures (fun h0 _ h1 -> live h0 input /\ live h0 res /\
+        live h1 input /\ live h1 res /\ modifies_1 res h0 h1))
 let text_to_nat input len res =
     let num_words = get_size_nat len in
     let m = U32.((len -^ 1ul) %^ bn_bytes) in
     text_to_nat_loop input len res num_words m 0uL 0ul
 
+(*
 val nat_to_text_loop:
-    input:bignum -> res:uint8_p -> i:U32.t ->
+    input:bignum -> res:uint8_p -> i:U32.t{U32.(v (i /^ bn_bytes)) <= length input} ->
     j:U32.t{U32.v j <= length res} -> Stack unit
 	(requires (fun h -> live h input /\ live h res))
-	(ensures (fun h0 _ h1 -> live h0 input /\ live h0 res /\ live h1 res /\ modifies_1 res h0 h1))
+	(ensures (fun h0 _ h1 -> live h0 input /\ live h0 res /\ 
+        live h1 input /\ live h1 res /\ modifies_1 res h0 h1))
 let rec nat_to_text_loop input res i j =
     if U32.(i >^ 0ul) then
-    let i = U32.(i -^ 1ul) in
-    let ind = U32.(i /^ bn_bytes) in
-    let l = input.(ind) in
-    let tmp = U32.(i %^ bn_bytes) in (* a bug in F* ? *)
-    res.(j) <- U8.(uint64_to_uint8 (U64.(l >>^ U32.(8ul *^ tmp))) &^ 0xffuy);
-    nat_to_text_loop input res i U32.(j +^ 1ul)
+        let i = U32.(i -^ 1ul) in
+        let ind = U32.(i /^ bn_bytes) in
+        let l = input.(ind) in
+        let tmp = U32.(i %^ bn_bytes) in
+        res.(j) <- U8.(uint64_to_uint8 (U64.(l >>^ U32.(8ul *^ tmp))) &^ 0xffuy);
+        let j = U32.(j +^ 1ul) in
+        nat_to_text_loop input res i j
     else ()
 
 val nat_to_text:
     input:bignum -> len:U32.t -> res:uint8_p{length res = U32.v len} -> Stack unit
 	(requires (fun h -> live h input /\ live h res))
-	(ensures (fun h0 _ h1 -> live h0 input /\ live h0 res /\ live h1 res /\ modifies_1 res h0 h1))
+	(ensures (fun h0 _ h1 -> live h0 input /\ live h0 res /\ 
+        live h1 input  /\ live h1 res /\ modifies_1 res h0 h1))
 let nat_to_text input len res =
     nat_to_text_loop input res len 0ul
+    *)
