code/experimental/rsa/Exponentiation.fst
@@ -7,6 +7,7 @@ open FStar.All
 
 open Multiplication
 open Division
+open Convert
 
 module U32 = FStar.UInt32
 module U64 = FStar.UInt64
@@ -31,41 +32,52 @@ let bn_bit_is_set input ind =
 
 val mod_exp_loop:
     modBits:U32.t -> aLen:U32.t -> bBits:U32.t -> resLen:U32.t ->
-    n:bignum -> tmpV:bignum{U32.v aLen = length tmpV} -> b:bignum ->
-    res:bignum{U32.v resLen = length res} -> count:U32.t{U32.v count < length b} -> Stack unit
+    n:bignum{length n = U32.v (bits_to_bn modBits)} -> 
+    tmpV:bignum{U32.v aLen = length tmpV} -> 
+    b:bignum{length b = U32.v (bits_to_bn bBits)} ->
+    res:bignum{U32.v resLen = length res} -> 
+    count:U32.t{U32.v count <= length b} -> Stack unit
     (requires (fun h -> live h n /\ live h tmpV /\ live h b /\ live h res))
-    (ensures  (fun h0 r h1 -> live h1 n /\ live h1 tmpV /\ live h1 b /\ live h1 res /\ modifies_1 res h0 h1 /\ modifies_1 tmpV h0 h1))
+    (ensures  (fun h0 r h1 -> live h0 n /\ live h0 tmpV /\ live h0 b /\ live h0 res /\
+        live h1 n /\ live h1 tmpV /\ live h1 b /\ live h1 res /\ 
+        modifies_1 res h0 h1 /\ modifies_1 tmpV h0 h1))
 let rec mod_exp_loop modBits aLen bBits resLen n tmpV b res count =
     push_frame();
     let tmpLen = U32.(2ul *^ aLen) in
     let tmp = create 0uL tmpLen in
     let tmpBits = U32.(tmpLen *^ 64ul) in
+    
     let tmpLen2 = U32.(aLen +^ resLen) in
     let tmp2 = create 0uL tmpLen2 in
     let tmpBits2 = U32.(tmpLen2 *^ 64ul) in
+    
     (if U32.(count <^ bBits) then
-        (sqr aLen tmpV tmp;
+       (sqr aLen tmpV tmp;
         remainder tmpBits modBits aLen tmp n tmpV;
-        (if (bn_bit_is_set b count) then
-        (mult resLen aLen res tmpV tmp2;
-        remainder tmpBits2 modBits resLen tmp2 n res));
-        mod_exp_loop modBits aLen bBits resLen n tmpV b res U32.(count +^ 1ul)));
+       (if (bn_bit_is_set b count) then
+           (mult resLen aLen res tmpV tmp2;
+            remainder tmpBits2 modBits resLen tmp2 n res));
+        let count = U32.(count +^ 1ul) in
+        mod_exp_loop modBits aLen bBits resLen n tmpV b res count));
     pop_frame()
 
 (* res = a ^^ b mod n *)
 val mod_exp:
     modBits:U32.t -> aLen:U32.t -> bBits:U32.t -> resLen:U32.t ->
-    n:bignum -> a:bignum{U32.v aLen = length a} -> b:bignum ->
+    n:bignum{length n = U32.v (bits_to_bn modBits)} ->
+    a:bignum{U32.v aLen = length a} ->
+    b:bignum{length b = U32.v (bits_to_bn bBits)} ->
     res:bignum{U32.v resLen = length res} -> Stack unit
     (requires (fun h -> live h n /\ live h a /\ live h b /\ live h res))
-    (ensures  (fun h0 r h1 -> live h1 n /\ live h1 a /\ live h1 b /\ live h1 res /\ modifies_1 res h0 h1))
+    (ensures  (fun h0 r h1 -> live h0 n /\ live h0 a /\ live h0 b /\ live h0 res /\
+        live h1 res /\ modifies_1 res h0 h1))
 let mod_exp modBits aLen bBits resLen n a b res =
     push_frame();
     let tmpV = create 0uL aLen in
     blit a 0ul tmpV 0ul aLen;
 
     if (bn_bit_is_set b 0ul) then
-    blit a 0ul res 0ul aLen
+        blit a 0ul res 0ul aLen
     else res.(0ul) <- 1uL;
 
     mod_exp_loop modBits aLen bBits resLen n b res tmpV 1ul;
