code/experimental/rsa/Division.fst
@@ -21,7 +21,8 @@ val remainder_loop:
     r_i:bignum{length r_i = U32.v rLen} -> mod:bignum{length mod = U32.v modLen} ->
     count:U32.t -> res:bignum{length res = U32.v resLen} -> Stack unit
     (requires (fun h -> live h r_i /\ live h mod /\ live h res))
-	(ensures (fun h0 _ h1 -> live h0 r_i /\ live h0 mod /\  live h0 res /\ live h1 res /\ modifies_1 res h0 h1))
+	(ensures (fun h0 _ h1 -> live h0 r_i /\ live h0 mod /\  live h0 res /\ 
+        live h1 res /\ modifies_1 res h0 h1))
 let rec remainder_loop rLen modLen resLen r_i mod count res =
     push_frame();
     let isSet = if U64.(mod.(U32.(modLen -^ 1ul)) =^ 1uL) then 1ul else 0ul in
@@ -29,12 +30,11 @@ let rec remainder_loop rLen modLen resLen r_i mod count res =
     let mod1 = create 0uL mod1Len in
     let tmp = create 0uL rLen in
     (if U32.(count >^ 0ul) then
-    (rshift1 modLen mod mod1;
-    if not (isMore modLen rLen mod r_i) then
-		(sub rLen modLen r_i mod tmp; blit tmp 0ul r_i 0ul rLen;
-		remainder_loop rLen mod1Len resLen r_i mod1 U32.(count -^ 1ul) res)
-	else
-		remainder_loop rLen mod1Len resLen r_i mod1 U32.(count -^ 1ul) res)
+       (rshift1 modLen mod mod1;
+        if not (isMore modLen rLen mod r_i) then
+		   (sub rLen modLen r_i mod tmp; blit tmp 0ul r_i 0ul rLen;
+		    remainder_loop rLen mod1Len resLen r_i mod1 U32.(count -^ 1ul) res)
+	    else remainder_loop rLen mod1Len resLen r_i mod1 U32.(count -^ 1ul) res)
     else
         let len = if U32.(resLen >^ rLen) then rLen else resLen in
         blit r_i 0ul res 0ul len);
@@ -47,7 +47,8 @@ val remainder:
     mod:bignum{length mod = U32.v (bits_to_bn modBits)} ->
     res:bignum{length res = U32.v resLen} -> Stack unit
 	(requires (fun h -> live h a /\ live h mod /\ live h res))
-	(ensures (fun h0 _ h1 -> live h0 a /\ live h0 mod /\  live h0 res /\ live h1 res /\ modifies_1 res h0 h1))
+	(ensures (fun h0 _ h1 -> live h0 a /\ live h0 mod /\  live h0 res /\ 
+        live h1 res /\ modifies_1 res h0 h1))
 let remainder aBits modBits resLen a mod res =
     push_frame();
     let aLen = bits_to_bn aBits in
