code/experimental/rsa/Shift.fst
@@ -17,64 +17,62 @@ val lshift_loop:
     a:bignum -> count:U32.t{U32.v count <= length a} -> nw:U32.t ->
     lb:U32.t -> res:bignum{U32.(v (count +^ nw)) < length res} -> Stack unit
 	(requires (fun h -> live h a /\ live h res))
-	(ensures (fun h0 _ h1 -> live h0 a /\ live h0 res /\ live h1 res /\ modifies_1 res h0 h1))
+	(ensures (fun h0 _ h1 -> live h0 a /\ live h0 res /\ 
+        live h1 a /\ live h1 res /\ modifies_1 res h0 h1))
 let rec lshift_loop a count nw lb res =
-    push_frame();
-    (if U32.(count >^ 0ul) then
-    let count = U32.(count -^ 1ul) in
-    let l = a.(count) in
-    let ind = U32.(nw +^ count +^ 1ul) in
-    let rb = U32.(bn_bits2 -^ lb) in
-    let tmp = res.(ind) in
-    res.(ind) <- U64.(tmp |^ ((l >>^ rb) &^ bn_mask2));
-    res.(U32.(ind -^ 1ul)) <- U64.((l <<^ lb) &^ bn_mask2);
-    lshift_loop a count nw lb res);
-    pop_frame()
+    if U32.(count >^ 0ul) then
+        let count = U32.(count -^ 1ul) in
+        let l = a.(count) in
+        let ind = U32.(nw +^ count +^ 1ul) in
+        let rb = U32.(bn_bits2 -^ lb) in
+        let tmp = res.(ind) in
+        res.(ind) <- U64.(tmp |^ ((l >>^ rb) &^ bn_mask2));
+        res.(U32.(ind -^ 1ul)) <- U64.((l <<^ lb) &^ bn_mask2);
+        lshift_loop a count nw lb res
+    else ()
 
 (* res = a << n *)
 val lshift:
     aLen:U32.t -> a:bignum{length a = U32.v aLen} -> nCount:U32.t ->
     res:bignum{length res = U32.(v (aLen +^ (nCount /^ bn_bits2) +^ 1ul))} -> Stack unit
 	(requires (fun h -> live h a /\ live h res))
-	(ensures (fun h0 _ h1 -> live h0 a /\ live h0 res /\ live h1 res /\ modifies_1 res h0 h1))
+	(ensures (fun h0 _ h1 -> live h0 a /\ live h0 res /\ 
+        live h1 a /\ live h1 res /\ modifies_1 res h0 h1))
 let lshift aLen a nCount res =
-    push_frame();
     let nw = U32.(nCount/^ bn_bits2) in
     let resLen = U32.(aLen +^ nw) in
     let lb = U32.(nCount %^ bn_bits2) in
-    (if U32.(lb =^ 0ul)
-    then blit a 0ul res nw aLen
-    else lshift_loop a aLen nw lb res);
-    pop_frame()
+    (if U32.(lb =^ 0ul) then 
+        blit a 0ul res nw aLen
+    else lshift_loop a aLen nw lb res)
 
 val rshift1_loop:
     a:bignum -> carry:U64.t -> ind:U32.t{U32.v ind <= length a} ->
     res:bignum{U32.v ind <= length res} -> Stack unit
     (requires (fun h -> live h a /\ live h res))
-	(ensures (fun h0 _ h1 -> live h0 a /\ live h0 res /\ live h1 res /\ modifies_1 res h0 h1))
+	(ensures (fun h0 _ h1 -> live h0 a /\ live h0 res /\ 
+        live h1 a /\ live h1 res /\ modifies_1 res h0 h1))
 let rec rshift1_loop a carry ind res =
-    push_frame();
-    (if U32.(ind >^ 0ul) then
-    let ind = U32.(ind -^ 1ul) in
-    let tmp = a.(ind) in
-    res.(ind) <- U64.(((tmp >>^ 1ul) &^ bn_mask2) |^ carry);
-    let carry = if U64.((tmp &^ 1uL) =^ 1uL) then bn_tbit else 0uL in
-    rshift1_loop a carry ind res);
-    pop_frame()
+    if U32.(ind >^ 0ul) then
+        let ind = U32.(ind -^ 1ul) in
+        let tmp = a.(ind) in
+        res.(ind) <- U64.(((tmp >>^ 1ul) &^ bn_mask2) |^ carry);
+        let carry = if U64.((tmp &^ 1uL) =^ 1uL) then bn_tbit else 0uL in
+        rshift1_loop a carry ind res
+    else ()
 
 (* res = a >> 1 *)
 val rshift1:
     aLen:U32.t -> a:bignum{length a = U32.v aLen} ->
     res:bignum{length res = U32.v aLen /\ length res = U32.(v (aLen -^ 1ul))} -> Stack unit
 	(requires (fun h -> live h a /\ live h res))
-	(ensures (fun h0 _ h1 -> live h0 a /\ live h0 res /\ live h1 res /\ modifies_1 res h0 h1))
+	(ensures (fun h0 _ h1 -> live h0 a /\ live h0 res /\ 
+        live h1 a /\ live h1 res /\ modifies_1 res h0 h1))
 let rshift1 aLen a res =
     (* if a = 0 then res = 0 *)
-    push_frame();
     let i = U32.(aLen -^ 1ul) in
     let tmp = a.(i) in
     let carry = if U64.((tmp &^ 1uL) =^ 1uL) then bn_tbit else 0uL in
     let tmp = U64.(tmp >>^ 1ul) in
     (if U64.(tmp >^ 0uL) then res.(i) <- tmp);
-    rshift1_loop a carry i res;
-    pop_frame()
+    rshift1_loop a carry i res
